wip prove proves' implies proves

candle/standard/syntax/littleTheoriesSyntaxScript.sml
@@ -17,13 +17,38 @@ Overload elimsigof = ``(λ(_, (c, _)). c):thy'->sig``
 Overload elimaxsof = ``(λ(_, (_, d)). d):thy'->term set``
 Overload tysof = ``tysof o sigof``
 Overload tmsof = ``tmsof o sigof``
+Overload etysof = ``tysof o elimsigof``
+Overload etmsof = ``tmsof o elimsigof``
 
 (* Standard signature includes the minimal type operators and constants *)
 
+(* term_ok' has to check if types are valid through both the types and
+ eliminable types *)
+Definition term_ok'_def:
+  (term_ok' (sig:sig) (esig:sig) (Var x ty) ⇔
+     type_ok (FUNION (tysof sig) (tysof esig)) ty) ∧
+  (term_ok' sig esig (Const name ty) ⇔
+     ∃ty0. FLOOKUP (FUNION (tmsof sig) (tmsof esig)) name = SOME ty0 ∧
+           type_ok (FUNION (tysof sig) (tysof esig)) ty ∧
+           is_instance ty0 ty) ∧
+  (term_ok' sig esig (Comb tm1 tm2) ⇔
+     term_ok' sig esig tm1 ∧
+     term_ok' sig esig tm2 ∧
+     welltyped (Comb tm1 tm2)) ∧
+  (term_ok' sig esig (Abs v tm) ⇔
+     ∃x ty.
+       v = Var x ty ∧
+       type_ok (FUNION (tysof sig) (tysof esig)) ty ∧
+       term_ok' sig esig tm)
+End
+
 Definition theory_ok'_def:
   theory_ok' (thy:thy') ⇔
-    (∀ty. ty ∈ FRANGE (tmsof thy) ⇒ type_ok (tysof thy) ty) ∧
+    (∀ty. ty ∈ FRANGE (tmsof thy) ⇒ type_ok (FUNION (tysof thy) (etysof thy)) ty) ∧
+    (∀ty. ty ∈ FRANGE (etmsof thy) ⇒ type_ok (FUNION (tysof thy) (etysof thy)) ty) ∧
     (∀p. p ∈ (axsof thy) ⇒ term_ok (sigof thy) p ∧ p has_type Bool) ∧
+    (∀p. p ∈ (elimaxsof thy) ⇒
+         term_ok' (sigof thy) (elimsigof thy) p ∧ p has_type Bool) ∧
     is_std_sig (sigof thy)
 End
 
@@ -33,24 +58,25 @@ val _ = Parse.add_infix("|-'",450,Parse.NONASSOC)
 
 Inductive proves':
 [~ABS:]
-  (¬(EXISTS (VFREE_IN (Var x ty)) h) ∧ type_ok (tysof thy) ty ∧
+  (¬(EXISTS (VFREE_IN (Var x ty)) h) ∧ type_ok (FUNION (tysof thy) (etysof thy)) ty ∧
    (thy, es, h) |-' l === r
    ⇒ (thy, es, h) |-' (Abs (Var x ty) l) === (Abs (Var x ty) r))
 
 [~ASSUME:]
-  (theory_ok' thy ∧ p has_type Bool ∧ term_ok (sigof thy) p
+  (theory_ok' thy ∧ p has_type Bool ∧ term_ok' (sigof thy) (elimsigof thy) p
    ⇒ (thy, es, [p]) |-' p)
 
 [~BETA:]
-  (theory_ok' thy ∧ type_ok (tysof thy) ty ∧ term_ok (sigof thy) t
+  (theory_ok' thy ∧ type_ok (FUNION (tysof thy) (etysof thy)) ty
+   ∧ term_ok' (sigof thy) (elimsigof thy) t
    ⇒ (thy, es, []) |-' Comb (Abs (Var x ty) t) (Var x ty) === t)
 
 [~DEDUCT_ANTISYM:]
   ((thy, es, h1) |-' c1 ∧
    (thy, es, h2) |-' c2
    ⇒ (thy, es, term_union (term_remove c2 h1)
-                      (term_remove c1 h2))
-           |-' c1 === c2)
+                          (term_remove c1 h2))
+     |-' c1 === c2)
 
 [~EQ_MP:]
   ((thy, es, h1) |-' p === q ∧
@@ -59,12 +85,13 @@ Inductive proves':
 
 [~INST:]
   ((∀s s'. MEM (s',s) ilist ⇒
-             ∃x ty. (s = Var x ty) ∧ s' has_type ty ∧ term_ok (sigof thy) s') ∧
+           ∃x ty. (s = Var x ty) ∧ s' has_type ty
+                  ∧ term_ok' (sigof thy) (elimsigof thy) s') ∧
    (thy, es, h) |-' c
    ⇒ (thy, es, term_image (VSUBST ilist) h) |-' VSUBST ilist c)
 
 [~INST_TYPE:]
-  ((EVERY (type_ok (tysof thy)) (MAP FST tyin)) ∧
+  ((EVERY (type_ok (FUNION (tysof thy) (etysof thy))) (MAP FST tyin)) ∧
    (thy, es, h) |-' c
    ⇒ (thy, es, term_image (INST tyin) h) |-' INST tyin c)
 
@@ -75,7 +102,7 @@ Inductive proves':
    ⇒ (thy, es, term_union h1 h2) |-' Comb l1 l2 === Comb r1 r2)
 
 [~REFL:]
-  (theory_ok' thy ∧ term_ok (sigof thy) t
+  (theory_ok' thy ∧ term_ok' (sigof thy) (elimsigof thy) t
    ⇒ (thy, es, []) |-' t === t)
 
 [~axioms:]
@@ -112,15 +139,17 @@ Proof
 QED
 
 Theorem type_ok_imp_elim:
-  type_ok (tysof thy) ty ⇒ type_ok (tysof (thy, empty_elims)) ty
+  type_ok (tysof thy) ty ⇒
+    type_ok (tysof (thy,empty_elims) ⊌ etysof (thy,empty_elims)) ty
 Proof
-  Cases_on ‘thy’ >> simp[type_ok_def]
+  Cases_on ‘thy’ >> simp[type_ok_def, empty_elims_def]
 QED
 
 Theorem type_ok_imp_elim_rw:
-  type_ok (tysof (sigof thy)) ty ⇒ type_ok (tysof (thy, empty_elims)) ty
+  type_ok (tysof (sigof thy)) ty ⇒
+    type_ok (tysof (thy,empty_elims) ⊌ etysof (thy,empty_elims)) ty
 Proof
-  Cases_on ‘thy’ >> simp[type_ok_def]
+  Cases_on ‘thy’ >> simp[type_ok_def, empty_elims_def]
 QED
 
 Theorem type_ok_sigof_imp_elim:
@@ -139,8 +168,19 @@ QED
 Theorem theory_ok_imp_elim:
   theory_ok thy ⇒ theory_ok' (thy, empty_elims)
 Proof
-  Cases_on ‘thy’ >> rw[theory_ok'_def, term_ok_imp_elim, theory_sig_eq_elim,
-                       type_ok_sigof_imp_elim, theory_ok_def, is_std_sig_def]
+  Cases_on ‘thy’
+  >> rw[theory_ok'_def, term_ok_imp_elim, theory_sig_eq_elim,
+        type_ok_sigof_imp_elim, theory_ok_def, is_std_sig_def,
+        empty_elims_def, theory_ok_def]
+QED
+
+Theorem term_ok'_imp:
+  term_ok' (sigof (thy, empty_elims)) (elimsigof (thy, empty_elims)) c
+  ⇔ term_ok (sigof thy) c
+Proof
+  Cases_on ‘thy’ >> rw[empty_elims_def]
+  >> Induct_on ‘c’ >> rw[term_ok_def] >> gvs[term_ok'_def]
+  >> metis_tac[]
 QED
 
 Theorem term_ok_sigof_imp:
@@ -149,25 +189,38 @@ Proof
   Cases_on ‘thy’ >> rw[theory_sig_eq_elim]
 QED
 
-Theorem theory_ok'_imp_elim:
-  theory_ok' (thy, _) ⇒ theory_ok' (thy, empty_elims)
+Theorem etysof_nil:
+  etysof (thy, empty_elims) = FEMPTY
 Proof
-  Cases_on ‘thy’ >> simp[theory_ok'_def]
+  rw[empty_elims_def]
+QED
+
+Theorem tysof_eq_elim_union:
+  tysof (sigof thy) = tysof (thy,empty_elims) ⊌ etysof (thy,empty_elims)
+Proof
+  Cases_on ‘thy’ >> rw[empty_elims_def]
+QED
+
+Theorem type_ok_imp:
+  type_ok (tysof (s, empty_elims)) ty
+  ⇔ type_ok (FUNION (tysof (s, empty_elims)) (etysof (s, empty_elims))) ty
+Proof
+  Cases_on ‘s’ >> Cases_on ‘q’ >> rw[empty_elims_def]
 QED
 
 Theorem proves_imp_proves':
  ∀h. (thy, h) |- c ⇒ ((thy, empty_elims), [], h) |-' c
 Proof
   Induct_on ‘$|-’ >> rw[]
-  >- (irule proves'_ABS >> rw[type_ok_imp_elim_rw])
-  >- (irule proves'_ASSUME >> rw[theory_ok_imp_elim, term_ok_sigof_imp])
-  >- (irule proves'_BETA >> rw[theory_ok_imp_elim, term_ok_sigof_imp, type_ok_imp_elim])
+  >- (irule proves'_ABS >> simp[type_ok_imp_elim_rw])
+  >- (irule proves'_ASSUME >> rw[theory_ok_imp_elim, term_ok'_imp])
+  >- (irule proves'_BETA >> rw[theory_ok_imp_elim, term_ok'_imp, type_ok_imp_elim])
   >- (irule proves'_DEDUCT_ANTISYM >> rw[])
   >- (irule proves'_EQ_MP >> metis_tac[])
-  >- (irule proves'_INST >> metis_tac[theory_sig_eq_elim])
-  >- (irule proves'_INST_TYPE >> gvs[theory_sig_eq_elim] >> simp[])
+  >- (irule proves'_INST >> metis_tac[term_ok'_imp])
+  >- (irule proves'_INST_TYPE >> metis_tac[tysof_eq_elim_union])
   >- (irule proves'_MK_COMB >> rw[])
-  >- (irule proves'_REFL >> rw[theory_ok_imp_elim, term_ok_sigof_imp])
+  >- (irule proves'_REFL >> rw[theory_ok_imp_elim, term_ok'_imp])
   >- (irule proves'_axioms >> rw[axsof_elim_thy, theory_ok_imp_elim])
 QED
 
@@ -260,8 +313,15 @@ Proof
   >- (irule proves_ABS >> rw[] >> gvs[])
   >- (irule proves_ASSUME >> rw[] >> gvs[theory_ok_def] >> metis_tac[])
   >- (irule proves_BETA >> rw[] >> gvs[theory_ok_def] >> metis_tac[])
-  >- (irule proves_DEDUCT_ANTISYM >> rw[] >> gvs[] >> cheat)
-  >> cheat
+  >- (irule proves_DEDUCT_ANTISYM >> rw[])
+  >- (irule proves_EQ_MP >> metis_tac[])
+  >- (irule proves_INST >> rw[] >> gvs[])
+  >- (irule proves_INST_TYPE >> rw[] >> gvs[])
+  >- (irule proves_MK_COMB >> rw[] >> gvs[])
+  >- (irule proves_REFL >> rw[theory_ok_def, type_ok_def]
+      >> gvs[theory_ok_def, type_ok_def])
+  >- (irule proves_axioms >> rw[theory_ok_def, type_ok_def]
+      >> gvs[theory_ok_def, type_ok_def])
 QED
 
 Theorem axioms_eliminable:
@@ -287,24 +347,103 @@ Proof
 QED
 
 Definition insert_sig_def:
-  insert_sig (etms, etys) (tms, tys) = (tms FUNION etms, tys FUNION etys)
+  insert_sig (etys, etms) (((tys, tms), axs):thy)
+  = (((FUNION tys etys, FUNION tms etms), axs):thy)
 End
 
+Theorem insert_sig_type_ok:
+  type_ok (tysof (sigof (thy,esig,eaxs)) ⊌
+                 tysof (elimsigof (thy,esig,eaxs))) ty
+  ⇔ type_ok (tysof (sigof (insert_sig esig thy))) ty
+Proof
+  Cases_on ‘thy’ >> Cases_on ‘esig’ >> Cases_on ‘q’
+  >> rw[insert_sig_def]
+QED
+
+Theorem is_std_sig_ext:
+  is_std_sig (p, q) ⇒ is_std_sig (FUNION p p', FUNION q q')
+Proof
+  Induct_on ‘p’ >> rw[is_std_sig_def] >> gvs[is_std_sig_def]
+  >> Cases_on ‘FLOOKUP f1 k’ >> rw[FLOOKUP_FUNION]
+QED
+
+(* if everything in l is type_ok, then adding more types will
+ keep it ok *)
+Theorem every_type_ok_ext:
+  EVERY (λa. type_ok p a) l ⇒ EVERY (λa. type_ok (p ⊌ p') a) l
+Proof
+  cheat
+QED
+
+Theorem type_ok_ext:
+  type_ok p t ⇒ type_ok (FUNION p q) t
+Proof
+  Cases_on ‘t’ >> rw[type_ok_def] >> gvs[type_ok_def]
+  >> rw[FLOOKUP_FUNION, every_type_ok_ext]
+QED
+
+Theorem term_ok_ext:
+  term_ok (p, q) c ⇒ term_ok (FUNION p p', FUNION q q') c
+Proof
+  Induct_on ‘c’ >> rw[term_ok_def] >> gvs[term_ok_def]
+  >> rw[type_ok_ext] >> qexists ‘ty0’ >> rw[FLOOKUP_FUNION]
+  >> metis_tac[]
+QED
+
+Theorem insert_sig_theory_ok:
+  theory_ok' (thy,esig,eaxs) ⇒ theory_ok (insert_sig esig thy)
+Proof
+  Cases_on ‘esig’ >> Cases_on ‘thy’ >> Cases_on ‘q'’
+  >> rw[theory_ok_def, insert_sig_def] >> gvs[theory_ok'_def]
+  >- (drule_all IN_FRANGE_FUNION_suff >> rw[])
+  >- rw[term_ok_ext]
+  >- rw[is_std_sig_ext]
+QED
+
+Theorem term_ok'_imp_insert_sig:
+  term_ok' (sigof (thy',esig,eaxs)) (elimsigof (thy',esig,eaxs)) c
+  ⇒ term_ok (sigof (insert_sig esig thy')) c
+Proof
+  Induct_on ‘c’ >> Cases_on ‘thy'’ >> rw[term_ok_def] >> gvs[term_ok'_def]
+  >> Cases_on ‘esig’ >> Cases_on ‘q’ >> rw[insert_sig_def] >> gvs[] >> metis_tac[]
+QED
+
+Theorem insert_sig_every_type_ok:
+  EVERY (type_ok (tysof (sigof (thy',esig,eaxs)) ⊌
+                        tysof (elimsigof (thy',esig,eaxs)))) (MAP FST tyin)
+  ⇒ EVERY (type_ok (tysof (insert_sig esig thy'))) (MAP FST tyin)
+Proof
+  cheat
+QED
+
+Theorem insert_sig_axsof:
+  c ∈ axsof (thy, esig, eaxs) ⇒ c ∈ axsof (insert_sig esig thy)
+Proof
+  Cases_on ‘thy’ >> rw[] >> Cases_on ‘q’ >> Cases_on ‘q'’ >> Cases_on ‘esig’
+  >> rw[insert_sig_def]
+QED
+
 Theorem proves'_imp_proves:
-  ∀h. ((thy, (eaxs, esig)), [], h) |-' c ==> (insert_sig esig thy, h) |- c
+  ∀h thy esig eaxs c. ((thy, (esig, eaxs)), [], h) |-' c
+      ==> (insert_sig esig thy, h) |- c
 Proof
   Induct_on ‘$|-'’ >> rw[]
-  >- (irule proves_ABS >> Cases_on ‘thy’ >> rw[insert_sig_def] >> gvs[])
-  >- (irule proves_ASSUME >> Cases_on ‘thy’ >> rw[insert_sig_def, theory_ok'_imp_elim])
-  >- (irule proves_BETA >> cheat)
-  >- (irule proves_DEDUCT_ANTISYM >> cheat)
-  >- (irule proves_EQ_MP >> cheat)
-  >- (irule proves_INST >> cheat)
-  >- (irule proves_INST_TYPE >> cheat)
-  >- (irule proves_MK_COMB >> cheat)
-  >- (irule proves_REFL >> cheat)
-  >- (irule proves_axioms >> cheat)
+  >- (irule proves_ABS >> rw[insert_sig_def] >> metis_tac[insert_sig_type_ok])
+  >- (irule proves_ASSUME >> rw[term_ok'_imp_insert_sig]
+      >> metis_tac[insert_sig_theory_ok, term_ok'_imp_insert_sig])
+  >- (irule proves_BETA >> rw[] >> metis_tac[
+          insert_sig_theory_ok, term_ok'_imp_insert_sig, insert_sig_type_ok])
+  >- (irule proves_DEDUCT_ANTISYM >> rw[])
+  >- (irule proves_EQ_MP >> metis_tac[])
+  >- (irule proves_INST >> metis_tac[term_ok'_imp_insert_sig])
+  >- (irule proves_INST_TYPE >> metis_tac[insert_sig_every_type_ok])
+  >- (irule proves_MK_COMB >> rw[])
+  >- (irule proves_REFL >> rw[]
+      >> metis_tac[insert_sig_theory_ok, term_ok'_imp_insert_sig])
+  >- (irule proves_axioms >> rw[] >> metis_tac[insert_sig_theory_ok, insert_sig_axsof])
+  >> irule proves_EQ_MP >> qexistsl [‘c’, ‘c’] >> cheat
 QED
+
 
 (* A context is a sequence of updates *)
 
@@ -391,7 +530,7 @@ Overload axsof = ``λctxt. set (axiom_list ctxt)``
 
 val _ = export_rewrites["types_of_upd_def","consts_of_upd_def","axexts_of_upd_def"]
 
-  (* Now we can recover the theory associated with a context *)
+(* Now we can recover the theory associated with a context *)
 Overload thyof = ``λctxt:update list. (sigof ctxt, axsof ctxt)``
 
 (* Principles for extending the context *)
